src/LeanEVM/Instructions/Stack.lean
@@ -8,9 +8,9 @@ open Outcome
 -- ==================================================================
 
 @[simp]
-def PUSH (evm: Evm)(bs:Array u8) : Outcome :=
+def PUSH (evm: Evm)(bs:Array u8)(p:bs.data.length < 32) : Outcome :=
   -- Convert bytes into a word
-  let w := u256.from_bytes bs;
+  let w := u256.from_bytes bs p;
   -- Push word
   Ok (evm.push w)
 
